Flapjack/Test/Pipeline.lean
@@ -224,9 +224,7 @@ example :
 example :
     loopToWordProg ({ vars := [] } : WordContext)
       (.primitive [7, 8] .addCarry [2, 3, 4]) =
-      .seq (.assign 1 (.var 4))
-        (.seq (.inst (.arith (.addCarry 3 1 2 3 1)))
-          (.seq (.assign 8 (.var 1)) (.assign 7 (.var 3)))) := by
+      .inst (.arith (.addCarry 7 8 2 3 4)) := by
   simp [loopToWordProg, wordFindVar, lookupNatInfo]
 
 example [NeZero width] :
